refactor

EXPLICIT-REFS/proof.v
@@ -1,802 +1,610 @@
-Require Import Bool ZArith Arith String List Max Logic.Eqdep_dec Program.Equality.
+Require Import String.
+Require Import Bool ZArith Arith List Max.
+Require Import Logic.Eqdep_dec Program.Equality.
+Require Import Classical.
 Set Implicit Arguments.
 
-Notation "x <- e1 ; e2" :=
-  (match e1 with
-   | None => None
-   | Some x => e2
-   end)
-    (right associativity, at level 60).
-
-Hint Resolve eq_nat_dec.
-Hint Resolve lt_S_n lt_n_S.
-
-Ltac simplify :=
-  repeat
-    match goal with
-    | [ H1 : False |- _ ] => destruct H1
-    | [ |- True ] => constructor
-    | [ H1 : True |- _ ] => clear H1
-    | [ |- ~ _ ] => intro
-    | [ H1 : ~ ?P1, H2 : ?P1 |- _ ] => destruct (H1 H2)
-    | [ H1 : _ \/ _ |- _ ] => destruct H1
-    | [ |- _ /\ _ ] => constructor
-    | [ H1 : _ /\ _ |- _ ] => destruct H1
-    | [ H1 : exists _, _ |- _ ] => destruct H1
-    | [ |- forall _, _ ] => intro
-    | [ _ : ?X1 = ?X2 |- _ ] => subst X2 || subst X1
-    end.
-
-Ltac existT_inversion :=
-  repeat (
-      match goal with
-      | [ H : existT _ _ _ = existT _ _ _ |- _ ] => apply inj_pair2_eq_dec in H; auto
-      end); subst; eauto 10.
-
-Inductive expression : nat -> Set :=
-| Const : forall ctx, nat -> expression ctx
-| Diff : forall ctx, expression ctx -> expression ctx -> expression ctx
-| IsZero : forall ctx, expression ctx -> expression ctx
-| If : forall ctx, expression ctx -> expression ctx -> expression ctx -> expression ctx
-| Var : forall ctx n, n < ctx -> expression ctx
-| Let : forall ctx, expression ctx -> expression (S ctx) -> expression ctx
-| Proc : forall ctx, expression (S ctx) -> expression ctx
-| Call : forall ctx, expression ctx -> expression ctx -> expression ctx
-| Newref : forall ctx, expression ctx -> expression ctx
-| Deref : forall ctx, expression ctx -> expression ctx
-| Setref : forall ctx, expression ctx -> expression ctx -> expression ctx.
-
-Lemma nltz : forall n, n < O -> False.
-  intro; omega.
-Qed.
-
-Definition partial_map (ctx : nat) (A : Type) := forall n, n < ctx -> A.
-Definition empty {A : Type} : partial_map O A.
-  refine (fun _ _ => match nltz _ with end);
-    eauto.
-Defined.
-Definition extend {ctx : nat} {A : Type} (v : A) (m : partial_map ctx A) : partial_map (S ctx) A.
-  refine (fun n =>
-            match n with
-            | O => fun _ => v
-            | S n' => fun _ => m _ _
-            end);
-    eauto.
-Defined.
+Definition var := string.
+Definition var_eq : forall x y : var, {x = y} + {x <> y} := string_dec.
+Infix "==v" := var_eq (no associativity, at level 50).
 
 Definition loc := nat.
+Definition loc_eq : forall x y : loc, {x = y} + {x <> y} := eq_nat_dec.
+Infix "==l" := loc_eq (no associativity, at level 50).
 
-Inductive expval : Type :=
-| Num : Z -> expval
-| Bool : bool -> expval
-| Clo : forall ctx, expression (S ctx) -> partial_map ctx expval -> expval
-| Ref : loc -> expval.
+Module ExplicitRefsSpec.
+  Inductive expression : Set :=
+  | ExpConst : nat -> expression
+  | ExpDiff : expression -> expression -> expression
+  | ExpIsZero : expression -> expression
+  | ExpIf : expression -> expression -> expression -> expression
+  | ExpVar : var -> expression
+  | ExpLet : var -> expression -> expression -> expression
+  | ExpProc : var -> expression -> expression
+  | ExpCall : expression -> expression -> expression
+  | ExpNewref : expression -> expression
+  | ExpDeref : expression -> expression
+  | ExpSetref : expression -> expression -> expression.
 
-Definition environment ctx := partial_map ctx expval.
-Definition empty_env : environment O := empty.
-Definition extend_env {ctx : nat} val env : partial_map (S ctx) expval := extend val env.
+  Implicit Type exp : expression.
 
-Definition store := loc -> option expval.
-Definition empty_store : store := fun _ => None.
-Definition extend_store l val st : store := fun q => if eq_nat_dec q l then Some val else st q.
+  Inductive expval : Set :=
+  | ValNum : Z -> expval
+  | ValBool : bool -> expval
+  | ValClo : var -> expression -> environment -> expval
+  | ValRef : loc -> expval
 
-Lemma extend_store_eq : forall l val st, (extend_store l val st) l = Some val.
-  intros.
-  unfold extend_store.
-  destruct (Nat.eq_dec l l); congruence.
-Qed.
+  with environment : Set :=
+       | EnvEmpty : environment
+       | EnvExtend : var -> expval -> environment -> environment.
 
-Lemma extend_store_neq : forall l q val st, q <> l -> (extend_store l val st) q = st q.
-  intros.
-  unfold extend_store.
-  destruct (Nat.eq_dec q l); congruence.
-Qed.
+  Implicit Type val : expval.
+  Implicit Type env : environment.
 
-Hint Resolve extend_store_eq extend_store_neq.
+  Inductive behavior : Set :=
+  | BehVal : expval -> behavior
+  | BehErr : behavior.
 
-Inductive value_of_rel: forall ctx, expression ctx -> environment ctx -> store -> expval -> store -> Prop :=
-| VConst :
-    forall ctx num env st,
-      value_of_rel (Const ctx num) env st (Num (Z.of_nat num)) st
-| VDiff :
-    forall ctx (exp1 : expression ctx) exp2 num1 num2 env st0 st1 st2,
-      value_of_rel exp1 env st0 (Num num1) st1 ->
-      value_of_rel exp2 env st1 (Num num2) st2 ->
-      value_of_rel (Diff exp1 exp2) env st0 (Num (num1 - num2)) st2
-| VIsZero :
-    forall ctx (exp1 : expression ctx) num1 env st0 st1,
-      value_of_rel exp1 env st0 (Num num1) st1 ->
-      value_of_rel (IsZero exp1) env st0 (Bool (Z.eqb num1 0)) st1
-| VIfTrue :
-    forall ctx (exp1 : expression ctx) exp2 exp3 val2 env st0 st1 st2,
-      value_of_rel exp1 env st0 (Bool true) st1 ->
-      value_of_rel exp2 env st1 val2 st2 ->
-      value_of_rel (If exp1 exp2 exp3) env st0 val2 st2
-| VIfFalse :
-    forall ctx (exp1 : expression ctx) exp2 exp3 val3 env st0 st1 st2,
-      value_of_rel exp1 env st0 (Bool false) st1 ->
-      value_of_rel exp3 env st1 val3 st2 ->
-      value_of_rel (If exp1 exp2 exp3) env st0 val3 st2
-| VVar :
-    forall ctx n (pf : n < ctx) env val st,
-      env _ pf = val ->
-      value_of_rel (Var pf) env st val st
-| VLet :
-    forall ctx (exp1 : expression ctx) body env val1 val st0 st1 st2,
-      value_of_rel exp1 env st0 val1 st1 ->
-      value_of_rel body (extend_env val1 env) st1 val st2 ->
-      value_of_rel (Let exp1 body) env st0 val st2
-| VProc :
-    forall ctx (body : expression (S ctx)) env st,
-      value_of_rel (Proc body) env st (Clo body env) st
-| VCall :
-    forall ctx (rator : expression ctx) rand env ctx' (body : expression (S ctx')) saved_env rand_val val st0 st1 st2 st3,
-      value_of_rel rator env st0 (Clo body saved_env) st1 ->
-      value_of_rel rand env st1 rand_val st2 ->
-      value_of_rel body (extend_env rand_val saved_env) st2 val st3 ->
-      value_of_rel (Call rator rand) env st0 val st3
-| VNewref :
-    forall ctx (exp1 : expression ctx) env val1 st0 st1 l,
-      value_of_rel exp1 env st0 val1 st1 ->
-      st1 l = None ->
-      value_of_rel (Newref exp1) env st0 (Ref l) (extend_store l val1 st1)
-| VDeref :
-    forall ctx (exp1 : expression ctx) env st0 st1 l val,
-      value_of_rel exp1 env st0 (Ref l) st1 ->
-      st1 l = Some val ->
-      value_of_rel (Deref exp1) env st0 val st1
-| VSetref :
-    forall ctx (exp1 : expression ctx) exp2 env st0 st1 st2 l val2 ori_val,
-      value_of_rel exp1 env st0 (Ref l) st1 ->
-      value_of_rel exp2 env st1 val2 st2 ->
-      st2 l = Some ori_val ->
-      value_of_rel (Setref exp1 exp2) env st0 (Num 23%Z) (extend_store l val2 st2).
+  Implicit Type beh : behavior.
 
-Lemma value_of_rel_const_inversion :
-  forall ctx num env val st0 st1,
-    value_of_rel (Const ctx num) env st0 val st1 ->
-    val = Num (Z.of_nat num) /\ st0 = st1.
-Proof.
-  intros.
-  inversion H.
-  existT_inversion.
-Qed.
+  Coercion BehVal : expval >-> behavior.
 
-Lemma value_of_rel_diff_inversion :
-  forall ctx (exp1 : expression ctx) exp2 env val st0 st2,
-    value_of_rel (Diff exp1 exp2) env st0 val st2 ->
-    exists num1 num2 st1,
-      value_of_rel exp1 env st0 (Num num1) st1 /\
-      value_of_rel exp2 env st1 (Num num2) st2 /\
-      val = Num (num1 - num2).
-Proof.
-  intros.
-  inversion H.
-  existT_inversion.
-Qed.
+  Definition empty_env := EnvEmpty.
+  Definition extend_env (env : environment) (x : var) (v : expval) := EnvExtend x v env.
+  Fixpoint apply_env (env : environment) (x : var) : behavior :=
+    match env with
+    | EnvEmpty => BehErr
+    | EnvExtend x' v env' => if x' ==v x then v else apply_env env' x
+    end.
 
-Lemma value_of_rel_is_zero_inversion :
-  forall ctx (exp1 : expression ctx) env val st0 st1,
-    value_of_rel (IsZero exp1) env st0 val st1 ->
-    exists num1,
-      value_of_rel exp1 env st0 (Num num1) st1 /\
-      val = Bool (Z.eqb num1 0).
-Proof.
-  intros.
-  inversion H.
-  existT_inversion.
-Qed.
+  Inductive term : Set :=
+  | TmExp : expression -> term
+  | TmDiff1 : behavior -> expression -> term
+  | TmDiff2 : expval -> behavior -> term
+  | TmIsZero1 : behavior -> term
+  | TmIf1 : behavior -> expression -> expression -> term
+  | TmLet1 : var -> behavior -> expression -> term
+  | TmCall1 : behavior -> expression -> term
+  | TmCall2 : expval -> behavior -> term
+  | TmNewref1 : behavior -> term
+  | TmDeref1 : behavior -> term
+  | TmSetref1 : behavior -> expression -> term
+  | TmSetref2 : expval -> behavior -> term.
 
-Lemma value_of_rel_if_inversion :
-  forall ctx (exp1 : expression ctx) exp2 exp3 env val st0 st2,
-    value_of_rel (If exp1 exp2 exp3) env st0 val st2 ->
-    exists st1,
-      (value_of_rel exp1 env st0 (Bool true) st1 /\ value_of_rel exp2 env st1 val st2) \/
-      (value_of_rel exp1 env st0 (Bool false) st1 /\ value_of_rel exp3 env st1 val st2).
-Proof.
-  intros.
-  inversion H;
-    existT_inversion.
-Qed.
+  Coercion TmExp : expression >-> term.
 
-Lemma value_of_rel_let_inversion :
-  forall ctx (exp1 : expression ctx) body env val st0 st2,
-    value_of_rel (Let exp1 body) env st0 val st2 ->
-    exists val1 st1,
-      value_of_rel exp1 env st0 val1 st1 /\
-      value_of_rel body (extend_env val1 env) st1 val st2.
-Proof.
-  intros.
-  inversion H.
-  existT_inversion.
-Qed.
+  Inductive abort : behavior -> Prop :=
+  | AbrErr : abort BehErr.
 
-Lemma value_of_rel_var_inversion :
-  forall ctx n (pf : n < ctx) env val st0 st1,
-    value_of_rel (Var pf) env st0 val st1 ->
-    exists (pf : n < ctx),
-      env _ pf = val /\ st0 = st1.
-Proof.
-  intros.
-  inversion H.
-  existT_inversion.
-Qed.
+  Inductive is_num : expval -> Prop :=
+  | IsNum : forall n, is_num (ValNum n).
 
-Lemma value_of_rel_proc_inversion :
-  forall ctx (body : expression (S ctx)) env val st0 st1,
-    value_of_rel (Proc body) env st0 val st1 ->
-    val = Clo body env /\ st0 = st1.
-Proof.
-  intros.
-  inversion H.
-  existT_inversion.
-Qed.
+  Inductive is_bool : expval -> Prop :=
+  | IsBool : forall b, is_bool (ValBool b).
 
-Lemma value_of_rel_call_inversion :
-  forall ctx (rator : expression ctx) rand env val st0 st3,
-    value_of_rel (Call rator rand) env st0 val st3 ->
-    exists ctx' (body : expression (S ctx')) saved_env rand_val st1 st2,
-      value_of_rel rator env st0 (Clo body saved_env) st1 /\
-      value_of_rel rand env st1 rand_val st2 /\
-      value_of_rel body (extend_env rand_val saved_env ) st2 val st3.
-Proof.
-  intros.
-  inversion H.
-  existT_inversion.
-Qed.
+  Inductive is_clo : expval -> Prop :=
+  | IsClo : forall x exp1 saved_env, is_clo (ValClo x exp1 saved_env).
 
-Lemma value_of_rel_newref_inversion :
-  forall ctx (exp1 : expression ctx) env val st0 st2,
-    value_of_rel (Newref exp1) env st0 val st2 ->
-    exists val1 l st1,
-      value_of_rel exp1 env st0 val1 st1 /\
-      val = Ref l /\ st1 l = None /\
-      st2 = extend_store l val1 st1.
-Proof.
-  intros.
-  inversion H.
-  existT_inversion.
-Qed.
+  Inductive is_ref : expval -> Prop :=
+  | IsRef : forall l, is_ref (ValRef l).
 
-Lemma value_of_rel_deref_inversion :
-  forall ctx (exp1 : expression ctx) env val st0 st1,
-    value_of_rel (Deref exp1) env st0 val st1 ->
-    exists l,
-      value_of_rel exp1 env st0 (Ref l) st1 /\
-      st1 l = Some val.
-Proof.
-  intros.
-  inversion H.
-  existT_inversion.
-Qed.
+  Definition store := list expval.
+  Definition empty_store : store := nil.
+  Definition newref_store (st : store) (val : expval) : store * loc :=
+    let l := length st in
+    (app st (cons val nil), l).
+  Definition deref_store (st : store) (l : loc) : behavior :=
+    match nth_error st l with
+    | Some val => val
+    | None => BehErr
+    end.
+  Definition setref_store (st : store) (l : loc) (val : expval) : option store :=
+    let inner :=
+        fix f (st : store) (l : loc) : option store :=
+          match st with
+          | nil => None
+          | val' :: st' =>
+            match l with
+            | O => Some (val :: st')
+            | S l' =>
+              match f st' l' with
+              | Some st' => Some (val' :: st')
+              | None => None
+              end
+            end
+          end in
+    inner st l.
 
-Lemma value_of_rel_setref_inversion :
-  forall ctx (exp1 : expression ctx) exp2 env val st0 st3,
-    value_of_rel (Setref exp1 exp2) env st0 val st3 ->
-    exists val2 l st1 st2 ori_val,
-      value_of_rel exp1 env st0 (Ref l) st1 /\
-      value_of_rel exp2 env st1 val2 st2 /\
-      st2 l = Some ori_val /\
-      st3 = extend_store l val2 st2.
-Proof.
-  intros.
-  inversion H.
-  existT_inversion.
-Qed.
+  Lemma deref_empty : forall l, deref_store empty_store l = BehErr.
+    intros; unfold deref_store, empty_store.
+    destruct l; simpl in *; eauto.
+  Qed.
 
-Definition naive_store_prop (sz : nat) (st : store) := forall l, (l < sz -> exists val, st l = Some val) /\ (l >= sz -> st l = None).
+  Inductive value_of_rel : environment -> term -> behavior -> store -> store -> Prop :=
+  | VrelConst :
+      forall env n st,
+        value_of_rel env (ExpConst n) (ValNum (Z.of_nat n)) st st
+  | VrelDiff :
+      forall env exp1 beh1 st0 st1 exp2 beh st2,
+        value_of_rel env exp1 beh1 st0 st1 ->
+        value_of_rel env (TmDiff1 beh1 exp2) beh st1 st2 ->
+        value_of_rel env (ExpDiff exp1 exp2) beh st0 st2
+  | VrefDiff1_abort :
+      forall beh1 env exp2 st,
+        abort beh1 ->
+        value_of_rel env (TmDiff1 beh1 exp2) beh1 st st
+  | VrelDiff1 :
+      forall env exp2 beh2 st0 st1 val1 beh st2,
+        value_of_rel env exp2 beh2 st0 st1 ->
+        value_of_rel env (TmDiff2 val1 beh2) beh st1 st2 ->
+        value_of_rel env (TmDiff1 val1 exp2) beh st0 st2
+  | VrelDiff2_abort :
+      forall beh2 env val1 st,
+        abort beh2 ->
+        value_of_rel env (TmDiff2 val1 beh2) beh2 st st
+  | VrelDiff2 :
+      forall env n1 n2 st,
+        value_of_rel env (TmDiff2 (ValNum n1) (ValNum n2)) (ValNum (n1 - n2)) st st
+  | VrelDiff2_err :
+      forall val1 val2 env st,
+        ~(is_num val1 /\ is_num val2) ->
+        value_of_rel env (TmDiff2 val1 val2) BehErr st st
+  | VrelIsZero :
+      forall env exp1 beh1 st0 st1 beh st2,
+        value_of_rel env exp1 beh1 st0 st1 ->
+        value_of_rel env (TmIsZero1 beh1) beh st1 st2 ->
+        value_of_rel env (ExpIsZero exp1) beh st0 st2
+  | VrelIsZero1_abort :
+      forall beh1 env st,
+        abort beh1 ->
+        value_of_rel env (TmIsZero1 beh1) beh1 st st
+  | VrelIsZero1 :
+      forall env n1 st,
+        value_of_rel env (TmIsZero1 (ValNum n1)) (ValBool (Z.eqb n1 0)) st st
+  | VrelIsZero1_err :
+      forall val1 env st,
+        ~is_num val1 ->
+        value_of_rel env (TmIsZero1 val1) BehErr st st
+  | VrelIf :
+      forall env exp1 beh1 st0 st1 exp2 exp3 beh st2,
+        value_of_rel env exp1 beh1 st0 st1 ->
+        value_of_rel env (TmIf1 beh1 exp2 exp3) beh st1 st2 ->
+        value_of_rel env (ExpIf exp1 exp2 exp3) beh st0 st2
+  | VrelIf1_abort :
+      forall beh1 env exp2 exp3 st,
+        abort beh1 ->
+        value_of_rel env (TmIf1 beh1 exp2 exp3) beh1 st st
+  | VrelIf1_true :
+      forall env exp2 beh2 st0 st1 exp3,
+        value_of_rel env exp2 beh2 st0 st1 ->
+        value_of_rel env (TmIf1 (ValBool true) exp2 exp3) beh2 st0 st1
+  | VrelIf1_false :
+      forall env exp3 beh3 st0 st1 exp2,
+        value_of_rel env exp3 beh3 st0 st1 ->
+        value_of_rel env (TmIf1 (ValBool false) exp2 exp3) beh3 st0 st1
+  | VrelIf1_err :
+      forall val1 env exp2 exp3 st,
+        ~is_bool val1 ->
+        value_of_rel env (TmIf1 val1 exp2 exp3) BehErr st st
+  | VrelVar :
+      forall env x st,
+        value_of_rel env (ExpVar x) (apply_env env x) st st
+  | VrelLet :
+      forall env exp1 beh1 st0 st1 x exp2 beh st2,
+        value_of_rel env exp1 beh1 st0 st1->
+        value_of_rel env (TmLet1 x beh1 exp2) beh st1 st2 ->
+        value_of_rel env (ExpLet x exp1 exp2) beh st0 st2
+  | VrelLet1_abort :
+      forall beh1 env x exp2 st,
+        abort beh1 ->
+        value_of_rel env (TmLet1 x beh1 exp2) beh1 st st
+  | VrelLet1 :
+      forall env x val1 exp2 beh2 st0 st1,
+        value_of_rel (extend_env env x val1) exp2 beh2 st0 st1 ->
+        value_of_rel env (TmLet1 x val1 exp2) beh2 st0 st1
+  | VrelProc :
+      forall env x exp1 st,
+        value_of_rel env (ExpProc x exp1) (ValClo x exp1 env) st st
+  | VrelCall :
+      forall env exp1 beh1 st0 st1 exp2 beh st2,
+        value_of_rel env exp1 beh1 st0 st1 ->
+        value_of_rel env (TmCall1 beh1 exp2) beh st1 st2 ->
+        value_of_rel env (ExpCall exp1 exp2) beh st0 st2
+  | VrelCall1_abort :
+      forall beh1 env exp2 st,
+        abort beh1 ->
+        value_of_rel env (TmCall1 beh1 exp2) beh1 st st
+  | VrelCall1 :
+      forall env exp2 beh2 st0 st1 val1 beh st2,
+        value_of_rel env exp2 beh2 st0 st1 ->
+        value_of_rel env (TmCall2 val1 beh2) beh st1 st2 ->
+        value_of_rel env (TmCall1 val1 exp2) beh st0 st2
+  | VrelCall2_abort :
+      forall beh2 env val1 st,
+        abort beh2 ->
+        value_of_rel env (TmCall2 val1 beh2) beh2 st st
+  | VrelCall2 :
+      forall saved_env x val2 exp1 beh st0 st1 env,
+        value_of_rel (extend_env saved_env x val2) exp1 beh st0 st1 ->
+        value_of_rel env (TmCall2 (ValClo x exp1 saved_env) val2) beh st0 st1
+  | VrelCall2_err :
+      forall val1 env val2 st,
+        ~is_clo val1 ->
+        value_of_rel env (TmCall2 val1 val2) BehErr st st
+  | VrelNewref :
+      forall env exp1 beh1 st0 st1 beh st2,
+        value_of_rel env exp1 beh1 st0 st1 ->
+        value_of_rel env (TmNewref1 beh1) beh st1 st2 ->
+        value_of_rel env (ExpNewref exp1) beh st0 st2
+  | VrelNewref1_abort :
+      forall beh1 env st,
+        abort beh1 ->
+        value_of_rel env (TmNewref1 beh1) beh1 st st
+  | VrelNewref1 :
+      forall st0 val1 st1 l env,
+        newref_store st0 val1 = (st1, l) ->
+        value_of_rel env (TmNewref1 val1) (ValRef l) st0 st1
+  | VrelDeref :
+      forall env exp1 beh1 st0 st1 beh st2,
+        value_of_rel env exp1 beh1 st0 st1 ->
+        value_of_rel env (TmDeref1 beh1) beh st1 st2 ->
+        value_of_rel env (ExpDeref exp1) beh st0 st2
+  | VrelDeref1_abort :
+      forall beh1 env st,
+        abort beh1 ->
+        value_of_rel env (TmDeref1 beh1) beh1 st st
+  | VrelDeref1 :
+      forall env l st,
+        value_of_rel env (TmDeref1 (ValRef l)) (deref_store st l) st st
+  | VrelSetref :
+      forall env exp1 beh1 st0 st1 exp2 beh st2,
+        value_of_rel env exp1 beh1 st0 st1 ->
+        value_of_rel env (TmSetref1 beh1 exp2) beh st1 st2 ->
+        value_of_rel env (ExpSetref exp1 exp2) beh st0 st2
+  | VrelSetref1_abort :
+      forall beh1 env exp2 st,
+        abort beh1 ->
+        value_of_rel env (TmSetref1 beh1 exp2) beh1 st st
+  | VrelSetref1 :
+      forall env exp2 beh2 st0 st1 val1 beh st2,
+        value_of_rel env exp2 beh2 st0 st1 ->
+        value_of_rel env (TmSetref2 val1 beh2) beh st1 st2 ->
+        value_of_rel env (TmSetref1 val1 exp2) beh st0 st2
+  | VrelSetref2_abort :
+      forall beh2 env val1 st,
+        abort beh2 ->
+        value_of_rel env (TmSetref2 val1 beh2) beh2 st st
+  | VrelSetref2 :
+      forall st0 l val st1 env,
+        setref_store st0 l val = Some st1 ->
+        value_of_rel env (TmSetref2 (ValRef l) val) (ValNum 23) st0 st1
+  | VrelSetref2_err1 :
+      forall val1 env val2 st,
+        ~is_ref val1 ->
+        value_of_rel env (TmSetref2 val1 val2) BehErr st st
+  | VrelSetref2_err2 :
+      forall st l val env,
+        setref_store st l val = None ->
+        value_of_rel env (TmSetref2 (ValRef l) val) BehErr st st.
 
-Definition naive_store (sz : nat) := { st : store | naive_store_prop sz st }.
+  Hint Constructors expression expval environment behavior term abort is_num is_bool is_clo is_ref value_of_rel.
+End ExplicitRefsSpec.
 
-Definition value_of : forall ctx sz, nat -> expression ctx -> naive_store sz -> environment ctx -> option (expval * { sz : nat & naive_store sz }).
-  refine (
-      fix F {ctx sz : nat} (fuel : nat) (exp : expression ctx) (st0 : naive_store sz) : environment ctx -> option (expval * { sz : nat & naive_store sz }) :=
-        match fuel with
-        | O => fun _ => None
-        | S fuel' =>
-          match exp with
-          | Const _ num => fun _ => Some (Num (Z.of_nat num), existT _ _ st0)
-          | Diff exp1 exp2 =>
-            fun env =>
-              ans1 <- F fuel' exp1 st0 env;
-              let (val1, ex1) := ans1 in
-              match ex1 with
-              | existT _ _ st1 =>
-                ans2 <- F fuel' exp2 st1 env;
-                let (val2, ex2) := ans2 in
+Module ExplicitRefsImpl.
+  Export ExplicitRefsSpec.
+
+  Implicit Type exp : expression.
+  Implicit Type val : expval.
+  Implicit Type env : environment.
+  Implicit Type beh : behavior.
+
+  Notation "x <-- e1 ; e2" :=
+    (match e1 with
+     | Some x => e2
+     | None => None
+     end)
+      (right associativity, at level 60).
+
+  Function value_of (fuel : nat) (env : environment) (exp : expression) (st : store) : option (behavior * store) :=
+    match fuel with
+    | O => None
+    | S fuel' =>
+      match exp with
+      | ExpConst n => Some (BehVal (ValNum (Z.of_nat n)), st)
+      | ExpDiff exp1 exp2 =>
+        res1 <-- value_of fuel' env exp1 st;
+          let (beh1, st1) := res1 in
+          match beh1 with
+          | BehVal val1 =>
+            res2 <-- value_of fuel' env exp2 st;
+              let (beh2, st2) := res2 in
+              match beh2 with
+              | BehVal val2 =>
                 match (val1, val2) with
-                | (Num num1, Num num2) => Some (Num (num1 - num2)%Z, ex2)
-                | _ => None
+                | (ValNum n1, ValNum n2) => Some (BehVal (ValNum (n1 - n2)), st2)
+                | _ => Some (BehErr, st2)
                 end
+              | BehErr => Some (BehErr, st2)
               end
-          | IsZero exp1 =>
-            fun env =>
-              ans1 <- F fuel' exp1 st0 env;
-              let (val1, ex1) := ans1 in
-              match val1 with
-              | Num num1 => Some (Bool (Z.eqb num1 0%Z), ex1)
-              | _ => None
-              end
-          | If exp1 exp2 exp3 =>
-            fun env =>
-              ans1 <- F fuel' exp1 st0 env;
-              let (val1, ex1) := ans1 in
-              match ex1 with
-              | existT _ _ st1 =>
-                match val1 with
-                | Bool true => F fuel' exp2 st1 env
-                | Bool false => F fuel' exp3 st1 env
-                | _ => None
-                end
-              end
-          | Var pf => fun env => Some (env _ pf, existT _ _ st0)
-          | Let exp1 body =>
-            fun env =>
-              ans1 <- F fuel' exp1 st0 env;
-              let (val1, ex1) := ans1 in
-              match ex1 with
-              | existT _ _ st1 => F fuel' body st1 (extend_env val1 env)
-              end
-          | Proc body => fun env => Some (Clo body env, existT _ _ st0)
-          | Call rator rand =>
-            fun env =>
-              ans1 <- F fuel' rator st0 env;
-              let (rator_val, ex1) := ans1 in
-              match ex1 with
-              | existT _ _ st1 =>
-                match rator_val with
-                | Clo body saved_env =>
-                  ans2 <- F fuel' rand st1 env;
-                  let (rand_val, ex2) := ans2 in
-                  match ex2 with
-                  | existT _ _ st2 => F fuel' body st2 (extend_env rand_val saved_env)
-                  end
-                | _ => None
-                end
-              end
-          | Newref exp1 =>
-            fun env =>
-              ans1 <- F fuel' exp1 st0 env;
-              let (val1, ex1) := ans1 in
-              match ex1 with
-              | existT _ sz1 st1 =>
-                match st1 with
-                | exist _ m1 pf1 => Some (Ref sz1, existT _ (S sz1) (exist _ (extend_store sz1 val1 m1) _))
-                end
-              end
-          | Deref exp1 =>
-            fun env =>
-              ans1 <- F fuel' exp1 st0 env;
-              let (val1, ex1) := ans1 in
-              match ex1 with
-              | existT _ sz1 st1 =>
-                match st1 with
-                | exist _ m1 _ => 
-                  match val1 with
-                  | Ref l1 =>
-                    match m1 l1 with
-                    | Some val => Some (val, ex1)
-                    | None => None
-                    end
-                  | _ => None
-                  end
-                end
-              end
-          | Setref exp1 exp2 =>
-            fun env =>
-              ans1 <- F fuel' exp1 st0 env;
-              let (val1, ex1) := ans1 in
-              match ex1 with
-              | existT _ sz1 st1 =>
-                match val1 with
-                | Ref l1 =>
-                  ans2 <- F fuel' exp2 st1 env;
-                  let (val2, ex2) := ans2 in
-                  match ex2 with
-                  | existT _ sz2 st2 =>
-                    if lt_dec l1 sz2 then
-                      match st2 with
-                      | exist _ m2 pf2 =>
-                        Some (Num 23%Z, existT _ sz2 (exist _ (extend_store l1 val2 m2) _))
-                      end
-                    else
-                      None
-                  end
-                | _ => None
-                end
-              end
+          | BehErr => Some (BehErr, st1)
           end
-        end).
-  intro.
-  specialize (pf1 l); simplify.
-  assert (l <= sz1). omega.
-  destruct H2.
-  eauto.
-  assert (l < S m). omega.
-  rewrite -> extend_store_neq; try omega.
-  eauto.
-  assert (l >= sz1). omega.
-  rewrite -> extend_store_neq; try omega.
-  auto.
+      | ExpIsZero exp1 =>
+        res1 <-- value_of fuel' env exp1 st;
+          let (beh1, st1) := res1 in
+          match beh1 with
+          | BehVal val1 =>
+            match val1 with
+            | ValNum n1 => Some (BehVal (ValBool (Z.eqb n1 0)), st1)
+            | _ => Some (BehErr, st1)
+            end
+          | BehErr => Some (BehErr, st1)
+          end
+      | ExpIf exp1 exp2 exp3 =>
+        res1 <-- value_of fuel' env exp1 st;
+          let (beh1, st1) := res1 in
+          match beh1 with
+          | BehVal val1 =>
+            match val1 with
+            | ValBool true => value_of fuel' env exp2 st1
+            | ValBool false => value_of fuel' env exp3 st1
+            | _ => Some (BehErr, st1)
+            end
+          | BehErr => Some (BehErr, st1)
+          end
+      | ExpVar x => Some (apply_env env x, st)
+      | ExpLet x exp1 exp2 =>
+        res1 <-- value_of fuel' env exp1 st;
+          let (beh1, st1) := res1 in
+          match beh1 with
+          | BehVal val1 =>
+            value_of fuel' (extend_env env x val1) exp2 st1
+          | BehErr => Some (BehErr, st1)
+          end
+      | ExpProc x exp1 => Some (BehVal (ValClo x exp1 env), st)
+      | ExpCall exp1 exp2 =>
+        res1 <-- value_of fuel' env exp1 st;
+          let (beh1, st1) := res1 in
+          match beh1 with
+          | BehVal val1 =>
+            res2 <-- value_of fuel' env exp2 st1;
+              let (beh2, st2) := res2 in
+              match beh2 with
+              | BehVal val2 =>
+                match val1 with
+                | ValClo x exp saved_env =>
+                  value_of fuel' (extend_env saved_env x val2) exp st2
+                | _ => Some (BehErr, st2)
+                end
+              | BehErr => Some (BehErr, st2)
+              end
+          | BehErr => Some (BehErr, st1)
+          end
+      | ExpNewref exp1 =>
+        res1 <-- value_of fuel' env exp1 st;
+          let (beh1, st1) := res1 in
+          match beh1 with
+          | BehVal val1 =>
+            let (st2, l) := newref_store st1 val1 in
+            Some (BehVal (ValRef l), st2)
+          | BehErr => Some (BehErr, st1)
+          end
+      | ExpDeref exp1 =>
+        res1 <-- value_of fuel' env exp1 st;
+          let (beh1, st1) := res1 in
+          match beh1 with
+          | BehVal val1 =>
+            match val1 with
+            | ValRef l => Some (deref_store st1 l, st1)
+            | _ => Some (BehErr, st1)
+            end
+          | BehErr => Some (BehErr, st1)
+          end
+      | ExpSetref exp1 exp2 =>
+        res1 <-- value_of fuel' env exp1 st;
+          let (beh1, st1) := res1 in
+          match beh1 with
+          | BehVal val1 =>
+            res2 <-- value_of fuel' env exp2 st1;
+              let (beh2, st2) := res2 in
+              match beh2 with
+              | BehVal val2 =>
+                match val1 with
+                | ValRef l =>
+                  match setref_store st2 l val2 with
+                  | Some st3 => Some (BehVal (ValNum 23), st3)
+                  | None => Some (BehErr, st2)
+                  end
+                | _ => Some (BehErr, st2)
+                end
+              | BehErr => Some (BehErr, st2)
+              end
+          | BehErr => Some (BehErr, st1)
+          end
+      end
+    end.
 
-  intro.
-  specialize (pf2 l0); simplify.
-  specialize (H H1).
-  destruct (Nat.eq_dec l0 l1); simplify.
-  rewrite -> extend_store_eq.
-  eauto.
-  rewrite -> extend_store_neq; auto.
-  eauto.
-  assert (l0 <> l1). omega.
-  rewrite -> extend_store_neq; auto.
-Defined.
+  Ltac invert' H := inversion H; clear H; subst.
 
-Ltac value_of_equation_finisher :=
-  repeat (
-      try match goal with
-          | [ H : value_of ?FUEL ?EXP ?ST ?ENV = _ |- context[match value_of ?FUEL ?EXP ?ST ?ENV with Some _ => _ | None => _ end] ] =>
-            try (rewrite -> H; clear H)
-          | [ H : ?LHS = ?RHS |- context[Some ?LHS = Some ?RHS] ] =>
-            rewrite -> H; clear H
-          | [ H : Some _ = Some _ |- _ ] =>
-            inversion H; subst; clear H
-          end;
-      simplify; eauto).
+  Theorem value_of_soundness :
+    forall env exp st0 beh st1,
+      (exists fuel, value_of fuel env exp st0 = Some (beh, st1)) ->
+      value_of_rel env exp beh st0 st1.
+  Proof.
+  Admitted.
 
-Lemma value_of_const_equation :
-  forall fuel ctx num env sz0 (st0 : naive_store sz0),
-    value_of (S fuel) (Const ctx num) st0 env = Some (Num (Z.of_nat num), existT _ _ st0).
-  intros.
-  simpl.
-  value_of_equation_finisher.
-Qed.
+  Definition value_of_term (fuel : nat) (env : environment) (tm : term) (st : store) : option (behavior * store) :=
+    match tm with
+    | TmExp exp => value_of fuel env exp st
+    | TmDiff1 beh1 exp2 =>
+      match beh1 with
+      | BehVal val1 =>
+        res2 <-- value_of fuel env exp2 st;
+          let (beh2, st2) := res2 in
+          match beh2 with
+          | BehVal val2 =>
+            match (val1, val2) with
+            | (ValNum n1, ValNum n2) => Some (BehVal (ValNum (n1 - n2)), st2)
+            | _ => Some (BehErr, st2)
+            end
+          | BehErr => Some (BehErr, st2)
+          end
+      | BehErr => Some (BehErr, st)
+      end
+    | TmDiff2 val1 beh2 =>
+      match beh2 with
+      | BehVal val2 =>
+        match (val1, val2) with
+        | (ValNum n1, ValNum n2) => Some (BehVal (ValNum (n1 - n2)), st)
+        | _ => Some (BehErr, st)
+        end
+      | BehErr => Some (BehErr, st)
+      end
+    | TmIsZero1 beh1 =>
+      match beh1 with
+      | BehVal val1 =>
+        match val1 with
+        | ValNum n1 => Some (BehVal (ValBool (Z.eqb n1 0)), st)
+        | _ => Some (BehErr, st)
+        end
+      | BehErr => Some (BehErr, st)
+      end
+    | TmIf1 beh1 exp2 exp3 =>
+      match beh1 with
+      | BehVal val1 =>
+        match val1 with
+        | ValBool true => value_of fuel env exp2 st
+        | ValBool false => value_of fuel env exp3 st
+        | _ => Some (BehErr, st)
+        end
+      | BehErr => Some (BehErr, st)
+      end
+    | TmLet1 x beh1 exp2 =>
+      match beh1 with
+      | BehVal val1 =>
+        value_of fuel (extend_env env x val1) exp2 st
+      | BehErr => Some (BehErr, st)
+      end
+    | TmCall1 beh1 exp2 =>
+      match beh1 with
+      | BehVal val1 =>
+        res2 <-- value_of fuel env exp2 st;
+          let (beh2, st2) := res2 in
+          match beh2 with
+          | BehVal val2 =>
+            match val1 with
+            | ValClo x exp saved_env =>
+              value_of fuel (extend_env saved_env x val2) exp st2
+            | _ => Some (BehErr, st2)
+            end
+          | BehErr => Some (BehErr, st2)
+          end
+      | BehErr => Some (BehErr, st)
+      end
+    | TmCall2 val1 beh2 =>
+      match beh2 with
+      | BehVal val2 =>
+        match val1 with
+        | ValClo x exp saved_env =>
+          value_of fuel (extend_env saved_env x val2) exp st
+        | _ => Some (BehErr, st)
+        end
+      | BehErr => Some (BehErr, st)
+      end
+    | TmNewref1 beh1 =>
+      match beh1 with
+      | BehVal val1 =>
+        let (st2, l) := newref_store st val1 in
+        Some (BehVal (ValRef l), st2)
+      | BehErr => Some (BehErr, st)
+      end
+    | TmDeref1 beh1 =>
+      match beh1 with
+      | BehVal val1 =>
+        match val1 with
+        | ValRef l => Some (deref_store st l, st)
+        | _ => Some (BehErr, st)
+        end
+      | BehErr => Some (BehErr, st)
+      end
+    | TmSetref1 beh1 exp2 =>
+      match beh1 with
+      | BehVal val1 =>
+        res2 <-- value_of fuel env exp2 st;
+          let (beh2, st2) := res2 in
+          match beh2 with
+          | BehVal val2 =>
+            match val1 with
+            | ValRef l =>
+              match setref_store st2 l val2 with
+              | Some st3 => Some (BehVal (ValNum 23), st3)
+              | None => Some (BehErr, st2)
+              end
+            | _ => Some (BehErr, st2)
+            end
+          | BehErr => Some (BehErr, st2)
+          end
+      | BehErr => Some (BehErr, st)
+      end
+    | TmSetref2 val1 beh2 =>
+      match beh2 with
+      | BehVal val2 =>
+        match val1 with
+        | ValRef l =>
+          match setref_store st l val2 with
+          | Some st3 => Some (BehVal (ValNum 23), st3)
+          | None => Some (BehErr, st)
+          end
+        | _ => Some (BehErr, st)
+        end
+      | BehErr => Some (BehErr, st)
+      end
+    end.
 
-Lemma value_of_diff_equation :
-  forall fuel ctx (exp1 : expression ctx) exp2 env num1 num2 sz0 (st0 : naive_store sz0) sz1 st1 sz2 st2,
-    value_of fuel exp1 st0 env = Some (Num num1, existT _ sz1 st1) ->
-    value_of fuel exp2 st1 env = Some (Num num2, existT _ sz2 st2) ->
-    value_of (S fuel) (Diff exp1 exp2) st0 env = Some (Num (num1 - num2), existT _ _ st2).
-Proof.
-  intros.
-  simpl.
-  value_of_equation_finisher.
-Qed.
+  Lemma le_max_1 : forall a b c, a <= max (max a b) c.
+    intros.
+    rewrite <- max_assoc.
+    apply le_max_l.
+  Qed.
 
-Lemma value_of_is_zero_equation :
-  forall fuel ctx (exp1 : expression ctx) env num1 sz0 (st0 : naive_store sz0) sz1 st1,
-    value_of fuel exp1 st0 env = Some (Num num1, existT _ sz1 st1) ->
-    value_of (S fuel) (IsZero exp1) st0 env = Some (Bool (Z.eqb num1 0), existT _ _ st1).
-Proof.
-  intros.
-  simpl.
-  value_of_equation_finisher.
-Qed.
+  Lemma le_max_2 : forall a b c, b <= max (max a b) c.
+    intros.
+    rewrite (max_comm a b).
+    rewrite <- max_assoc.
+    apply le_max_l.
+  Qed.
 
-Lemma value_of_if_true_equation :
-  forall fuel ctx (exp1 : expression ctx) exp2 exp3 env val sz0 (st0 : naive_store sz0) sz1 st1 sz2 st2,
-    value_of fuel exp1 st0 env = Some (Bool true, existT _ sz1 st1) ->
-    value_of fuel exp2 st1 env = Some (val, existT _ sz2 st2) ->
-    value_of (S fuel) (If exp1 exp2 exp3) st0 env = Some (val, existT _ _ st2).
-Proof.
-  intros.
-  simpl.
-  value_of_equation_finisher.
-Qed.
+  Lemma le_max_3 : forall a b c, c <= max (max a b) c.
+    intros.
+    apply le_max_r.
+  Qed.
 
-Lemma value_of_if_false_equation :
-  forall fuel ctx (exp1 : expression ctx) exp2 exp3 env val sz0 (st0 : naive_store sz0) sz1 st1 sz2 st2,
-    value_of fuel exp1 st0 env = Some (Bool false, existT _ sz1 st1) ->
-    value_of fuel exp3 st1 env = Some (val, existT _ sz2 st2) ->
-    value_of (S fuel) (If exp1 exp2 exp3) st0 env = Some (val, existT _ _ st2).
-Proof.
-  intros.
-  simpl.
-  value_of_equation_finisher.
-Qed.
+  Hint Resolve le_max_l le_max_r le_max_1 le_max_2 le_max_3.
 
-Lemma value_of_var_equation :
-  forall fuel ctx (env : environment ctx) n (pf : n < ctx) val sz0 (st0 : naive_store sz0),
-    env _ pf = val ->
-    value_of (S fuel) (Var pf) st0 env = Some (val, existT _ _ st0).
-Proof.
-  intros.
-  simpl.
-  value_of_equation_finisher.
-Qed.
+  Theorem value_of_term_completeness :
+    forall env tm beh st0 st1,
+      value_of_rel env tm beh st0 st1 ->
+      exists fuel, value_of_term fuel env tm st0 = Some (beh, st1).
+  Proof.
+  Admitted.
 
-Lemma value_of_let_equation :
-  forall fuel ctx (exp1 : expression ctx) body env val1 val sz0 (st0 : naive_store sz0) sz1 st1 sz2 st2,
-    value_of fuel exp1 st0 env = Some (val1, existT _ sz1 st1) ->
-    value_of fuel body st1 (extend_env val1 env) = Some (val, existT _ sz2 st2) ->
-    value_of (S fuel) (Let exp1 body) st0 env = Some (val, existT _ _ st2).
-Proof.
-  intros.
-  simpl.
-  value_of_equation_finisher.
-Qed.
+  Theorem value_of_completeness :
+    forall env exp beh st0 st1,
+      value_of_rel env exp beh st0 st1 ->
+      exists fuel, value_of fuel env exp st0 = Some (beh, st1).
+  Proof.
+    intros.
+    apply value_of_term_completeness in H; auto.
+  Qed.
 
-Lemma value_of_proc_equation :
-  forall fuel ctx (body : expression (S ctx)) (env : environment ctx) sz0 (st0 : naive_store sz0) env,
-    value_of (S fuel) (Proc body) st0 env = Some (Clo body env, existT _ _ st0).
-Proof.
-  intros.
-  simpl.
-  value_of_equation_finisher.
-Qed.
+  Hint Resolve value_of_soundness value_of_completeness.
 
-Lemma value_of_call_equation :
-  forall fuel ctx (rator : expression ctx) rand env rand_val val ctx' (body : expression (S ctx')) saved_env sz0 (st0 : naive_store sz0) sz1 st1 sz2 st2 sz3 st3,
-    value_of fuel rator st0 env = Some (Clo body saved_env, existT _ sz1 st1) ->
-    value_of fuel rand st1 env = Some (rand_val, existT _ sz2 st2) ->
-    value_of fuel body st2 (extend_env rand_val saved_env) = Some (val, existT _ sz3 st3) ->
-    value_of (S fuel) (Call rator rand) st0 env = Some (val, existT _ _ st3).
-Proof.
-  intros.
-  simpl.
-  value_of_equation_finisher.
-Qed.
+  Theorem value_of_correctness :
+    forall env exp st0 beh st1,
+      (exists fuel, value_of fuel env exp st0 = Some (beh, st1)) <->
+      value_of_rel env exp beh st0 st1.
+  Proof.
+    intuition.
+  Qed.
+End ExplicitRefsImpl.
 
-Lemma value_of_newref_equation :
-  forall fuel ctx (exp1 : expression ctx) env val1 sz0 (st0 : naive_store sz0) sz1 m1 pf1,
-    value_of fuel exp1 st0 env = Some (val1, existT _ sz1 (exist _ m1 pf1)) ->
-    exists pf1,
-      value_of (S fuel) (Newref exp1) st0 env = Some (Ref sz1, existT _ (S sz1) (exist _ (extend_store sz1 val1 m1) pf1)).
-Proof.
-  intros.
-  simpl.
-  value_of_equation_finisher.
-Qed.
-
-Lemma value_of_deref_equation :
-  forall fuel ctx (exp1 : expression ctx) env l1 sz0 (st0 : naive_store sz0) val sz1 m1 pf1,
-    value_of fuel exp1 st0 env = Some (Ref l1, existT _ sz1 (exist _ m1 pf1)) ->
-    m1 l1 = Some val ->
-    value_of (S fuel) (Deref exp1) st0 env = Some (val, existT _ _ (exist _ m1 pf1)).
-Proof.
-  intros.
-  simpl.
-  value_of_equation_finisher.
-  destruct (m1 l1); try discriminate.
-  value_of_equation_finisher.
-Qed.
-
-Lemma value_of_setref_equation :
-  forall fuel ctx (exp1 : expression ctx) exp2 env l1 val2 sz0 (st0 : naive_store sz0) sz1 st1 sz2 m2 pf2,
-    value_of fuel exp1 st0 env = Some (Ref l1, existT _ sz1 st1) ->
-    value_of fuel exp2 st1 env = Some (val2, existT _ sz2 (exist _ m2 pf2)) ->
-    l1 < sz2 ->
-    exists pf2,
-      value_of (S fuel) (Setref exp1 exp2) st0 env = Some (Num 23, existT _ sz2 (exist _ (extend_store l1 val2 m2) pf2)).
-Proof.
-  intros.
-  simpl.
-  value_of_equation_finisher.
-  destruct (lt_dec l1 sz2); try congruence.
-  value_of_equation_finisher.
-Qed.
-
-Hint Resolve value_of_const_equation value_of_diff_equation value_of_is_zero_equation value_of_if_true_equation value_of_if_false_equation value_of_var_equation value_of_let_equation value_of_proc_equation value_of_call_equation value_of_newref_equation value_of_deref_equation value_of_setref_equation.
-Hint Constructors value_of_rel.
-
-Theorem value_of_soundness :
-  forall ctx (exp : expression ctx) env val sz0 m0 (pf0 : naive_store_prop sz0 m0) sz1 m1 pf1,
-    (exists fuel, value_of fuel exp (exist _ m0 pf0) env = Some (val, existT _ sz1 (exist _ m1 pf1))) ->
-    value_of_rel exp env m0 val m1.
-Proof.
-  intros.
-  destruct H as [ fuel ? ].
-  generalize dependent ctx.
-  generalize dependent val.
-  generalize dependent sz0.
-  generalize dependent sz1.
-  generalize dependent m0.
-  generalize dependent m1.
-  induction fuel; try discriminate.
-  intros.
-  dependent destruction exp;
-    match goal with
-    | [ H : value_of ?FUEL ?EXP ?ST ?ENV = _ |- _ ] => simpl in H
-    end;
-    repeat (
-        try match goal with
-            | [ _ : context[match value_of ?FUEL ?EXP ?ST ?ENV with Some _ => _ | None => _ end] |- _ ] => destruct (value_of FUEL EXP ST ENV) eqn:?; try discriminate
-            | [ _ : context[let (_, _) := ?X in _] |- _ ] => destruct X
-            | [ _ : context[match ?VAL with Num _ => _ | Bool _ => _ | Clo _ _ => _ | Ref _ => _ end] |- _ ] => destruct VAL; try discriminate
-            | [ _ : context[if ?B then _ else _] |- _ ] => destruct B
-            | [ _ : context[match ?ST ?LOC with Some _ => _ | None => _ end] |- _ ] => destruct (ST LOC) eqn:?; try discriminate
-            | [ _ : context[match lt_dec ?X ?Y with left _ => _ | right _ => _ end] |- _ ] => destruct (lt_dec X Y); try discriminate
-            | [ st : naive_store _ |- _ ] => destruct st
-            | [ H : Some _ = Some _ |- _ ] => inversion H; clear H
-            | [ H : exist _ _ _ = exist _ _ _ |- _ ] => inversion H; clear H
-            | [ H : existT _ _ _ = existT _ _ _ |- _ ] => inversion H; clear H
-            end;
-        simplify;
-        eauto 10).
-  
-  assert (pf := n).
-  specialize (pf x).
-  simplify.
-  eauto.
-
-  assert (pf := n0).
-  specialize (pf l).
-  simplify.
-  apply H in l0.
-  simplify.
-  eauto.
-Qed.
-
-Lemma fuel_refl :
-  forall fuel ctx (exp : expression ctx) env val sz0 m0 (pf0 : naive_store_prop sz0 m0) sz1 m1 pf1,
-    value_of fuel exp (exist _ m0 pf0) env = Some (val, existT _ sz1 (exist _ m1 pf1)) ->
-    forall (pf0 : naive_store_prop sz0 m0), exists pf1,
-        value_of fuel exp (exist _ m0 pf0) env = Some (val, existT _ sz1 (exist _ m1 pf1)).
-Proof.
-  intros.
-  generalize dependent ctx.
-  generalize dependent val.
-  generalize dependent sz0.
-  generalize dependent sz1.
-  generalize dependent m0.
-  generalize dependent m1.
-  induction fuel; try discriminate.
-  intros.
-  dependent destruction exp;
-    match goal with
-    | [ H : value_of ?FUEL ?EXP ?ST ?ENV = _ |- _ ] => simpl in H
-    end;
-    repeat (
-        try match goal with
-            | [ _ : context[match value_of ?FUEL ?EXP ?ST ?ENV with Some _ => _ | None => _ end] |- _ ] => destruct (value_of FUEL EXP ST ENV) eqn:?; try discriminate
-            | [ _ : context[let (_, _) := ?X in _] |- _ ] => destruct X
-            | [ _ : context[match ?VAL with Num _ => _ | Bool _ => _ | Clo _ _ => _ | Ref _ => _ end] |- _ ] => destruct VAL; try discriminate
-            | [ _ : context[if ?B then _ else _] |- _ ] => destruct B
-            | [ _ : context[match ?ST ?LOC with Some _ => _ | None => _ end] |- _ ] => destruct (ST LOC) eqn:?; try discriminate
-            | [ _ : context[match lt_dec ?X ?Y with left _ => _ | right _ => _ end] |- _ ] => destruct (lt_dec X Y); try discriminate
-            | [ st : naive_store _ |- _ ] => destruct st
-            | [ H : Some _ = Some _ |- _ ] => inversion H; clear H
-            end;
-        simplify;
-        eauto 10).
-
-  apply IHfuel with (pf2 := pf2) in Heqo; auto; simplify.
-  apply IHfuel with (pf2 := x1) in Heqo0; auto; simplify.
-  eauto.
-
-  apply IHfuel with (pf2 := pf2) in Heqo; auto; simplify.
-  eauto.
-
-  apply IHfuel with (pf2 := pf2) in Heqo; auto; simplify.
-  apply IHfuel with (pf2 := x1) in H; auto; simplify.
-  eauto.
-
-  apply IHfuel with (pf2 := pf2) in Heqo; auto; simplify.
-  apply IHfuel with (pf2 := x1) in H; auto; simplify.
-  eauto.
-
-  apply IHfuel with (pf2 := pf2) in Heqo; auto; simplify.
-  apply IHfuel with (pf2 := x1) in H; auto; simplify.
-  eauto.
-
-  apply IHfuel with (pf2 := pf2) in Heqo; auto; simplify.
-  apply IHfuel with (pf2 := x3) in Heqo0; auto; simplify.
-  apply IHfuel with (pf2 := x4) in H; auto; simplify.
-  eauto.
-
-  apply IHfuel with (pf2 := pf2) in Heqo; auto; simplify.
-  eauto.
-
-  apply IHfuel with (pf2 := pf2) in Heqo; auto; simplify.
-  eauto.
-
-  apply IHfuel with (pf2 := pf2) in Heqo; auto; simplify.
-  apply IHfuel with (pf2 := x3) in Heqo0; auto; simplify.
-  eauto.
-Qed.
-
-Lemma fuel_incr :
-  forall fuel ctx (exp : expression ctx) env val sz0 m0 (pf0 : naive_store_prop sz0 m0) sz1 m1 pf1,
-    value_of fuel exp (exist _ m0 pf0) env = Some (val, existT _ sz1 (exist _ m1 pf1)) ->
-    forall (pf0 : naive_store_prop sz0 m0), exists pf1,
-        value_of (S fuel) exp (exist _ m0 pf0) env = Some (val, existT _ sz1 (exist _ m1 pf1)).
-Proof.
-  intros.
-  generalize dependent ctx.
-  generalize dependent val.
-  generalize dependent sz0.
-  generalize dependent sz1.
-  generalize dependent m1.
-  generalize dependent m0.
-  induction fuel; try discriminate.
-  intros.
-  dependent destruction exp;
-    match goal with
-    | [ H : value_of ?FUEL ?EXP ?ST ?ENV = _ |- _ ] => simpl in H
-    end;
-    repeat (
-        try match goal with
-            | [ _ : context[match value_of ?FUEL ?EXP ?ST ?ENV with Some _ => _ | None => _ end] |- _ ] => destruct (value_of FUEL EXP ST ENV) eqn:?; try discriminate
-            | [ _ : context[let (_, _) := ?X in _] |- _ ] => destruct X
-            | [ _ : context[match ?VAL with Num _ => _ | Bool _ => _ | Clo _ _ => _ | Ref _ => _ end] |- _ ] => destruct VAL; try discriminate
-            | [ _ : context[if ?B then _ else _] |- _ ] => destruct B
-            | [ _ : context[match ?ST ?LOC with Some _ => _ | None => _ end] |- _ ] => destruct (ST LOC) eqn:?; try discriminate
-            | [ _ : context[match lt_dec ?X ?Y with left _ => _ | right _ => _ end] |- _ ] => destruct (lt_dec X Y); try discriminate
-            | [ st : naive_store _ |- _ ] => destruct st
-            | [ H : Some _ = Some _ |- _ ] => inversion H; clear H
-            end;
-        simplify;
-        eauto 10).
-  
-  apply IHfuel with (pf2 := pf2) in Heqo; auto; simplify.
-  apply IHfuel with (pf2 := x1) in Heqo0; auto; simplify.
-  eauto.
-  
-  apply IHfuel with (pf2 := pf2) in Heqo; auto; simplify.
-  eauto.
-
-  apply IHfuel with (pf2 := pf2) in Heqo; auto; simplify.
-  apply IHfuel with (pf2 := x1) in H; auto; simplify.
-  eauto.
-
-  apply IHfuel with (pf2 := pf2) in Heqo; auto; simplify.
-  apply IHfuel with (pf2 := x1) in H; auto; simplify.
-  eauto.
-
-  apply IHfuel with (pf2 := pf2) in Heqo; auto; simplify.
-  apply IHfuel with (pf2 := x1) in H; auto; simplify.
-  eauto.
-
-  apply IHfuel with (pf2 := pf2) in Heqo; auto; simplify.
-  apply IHfuel with (pf2 := x3) in Heqo0; auto; simplify.
-  apply IHfuel with (pf2 := x4) in H; auto; simplify.
-  eauto.
-
-  apply IHfuel with (pf2 := pf2) in Heqo; auto; simplify.
-  eauto.
-
-  apply IHfuel with (pf2 := pf2) in Heqo; auto; simplify.
-  eauto.
-
-  apply IHfuel with (pf2 := pf2) in Heqo; auto; simplify.
-  apply IHfuel with (pf2 := x3) in Heqo0; auto; simplify.
-  eauto.
-Qed.
-
-Lemma fuel_order :
-  forall ctx (exp : expression ctx) env val fuel fuel' sz0 m0 (pf0 : naive_store_prop sz0 m0) sz1 m1 pf1,
-    value_of fuel exp (exist _ m0 pf0) env = Some (val, existT _ sz1 (exist _ m1 pf1)) ->
-    fuel <= fuel' ->
-    forall (pf0 : naive_store_prop sz0 m0), exists pf1,
-        value_of fuel' exp (exist _ m0 pf0) env = Some (val, existT _ sz1 (exist _ m1 pf1)).
-Proof.
-  Hint Resolve fuel_refl fuel_incr.
-  intros.
-  generalize dependent ctx.
-  generalize dependent val.
-  generalize dependent sz0.
-  generalize dependent m0.
-  generalize dependent sz1.
-  generalize dependent m1.
-  induction H0; intros.
-  eauto.
-  apply IHle with (pf2 := pf2) in H; auto; simplify.
-  eauto.
-Qed.
-
-Lemma le_max_1 : forall a b c, a <= max (max a b) c.
-  intros.
-  rewrite <- max_assoc.
-  apply le_max_l.
-Qed.
-
-Lemma le_max_2 : forall a b c, b <= max (max a b) c.
-  intros.
-  rewrite (max_comm a b).
-  rewrite <- max_assoc.
-  apply le_max_l.
-Qed.
-
-Lemma le_max_3 : forall a b c, c <= max (max a b) c.
-  intros.
-  apply le_max_r.
-Qed.
+Export ExplicitRefsImpl.
